Superposition_Calculus/Clausal_Calculus_Extra.thy
@@ -1,0 +1,24 @@
+theory Clausal_Calculus_Extra
+  imports "Saturation_Framework_Extensions.Clausal_Calculus" "Uprod_Extra"
+begin
+
+lemma map_literal_inverse: 
+  "(\<And>x. f (g x) = x) \<Longrightarrow> (\<And>literal. map_literal f (map_literal g literal) = literal)"
+  by (simp add: literal.map_comp literal.map_ident_strong)
+
+lemma map_literal_comp: 
+  "map_literal f (map_literal g literal) = map_literal (\<lambda>atom. f (g atom)) literal"
+  unfolding comp_def[symmetric]
+  by (simp add: literal.map_comp)
+
+lemma literals_distinct [simp]: "Neg \<noteq> Pos" "Pos \<noteq> Neg"
+  by(metis literal.distinct(1))+
+
+primrec mset_lit :: "'a uprod literal \<Rightarrow> 'a multiset" where
+  "mset_lit (Pos A) = mset_uprod A" |
+  "mset_lit (Neg A) = mset_uprod A + mset_uprod A"
+
+lemma mset_lit_image_mset: "mset_lit (map_literal (map_uprod f) l) = image_mset f (mset_lit l)"
+  by(induction l) (simp_all add: mset_uprod_image_mset)
+
+end
